do away with flat_function_type

theories/typechecker/typechecker.v
@@ -5186,45 +5186,80 @@ Fixpoint synth_possible_resulting_local_ctx_insts F insts L : (option local_ctx)
       end
   end.
 
+Fixpoint body_has_mono_type_checker
+  (M : module_ctx)
+  (K : kind_ctx)
+  (mf_locs : list representation)
+  (body : list instruction)
+  (κs : list kind)
+  (τs1 τs2 : list type)
+  : type_checker_res :=
+  match mapM (eval_rep_prim EmptyEnv) mf_locs with
+  | Some ηss_L =>
+      let tempF := Build_function_ctx [] [] [] K κs in
+      match mapM (grab_rep tempF) τs1 with
+      | Some ρs_P =>
+          match mapM (eval_rep_prim EmptyEnv) ρs_P with
+          | Some ηss_P =>
+              let tempF2 := Build_function_ctx τs2 (ηss_P ++ ηss_L) [] K κs in
+              let L := τs1 ++ map type_plug_prim ηss_L in
+              let ψ := InstrT [] τs2 in
+              match synth_possible_resulting_local_ctx_insts tempF2 body L with
+              | inl (Some L') =>
+                  let F := tempF2 <| fc_labels := [(τs2, L')] |> in
+                  let res := map (λ t, has_ref_flag_checker F t NoRefs) L' in
+                  let folded := foldr (λ r, andb (check_ok_output r)) true res in
+                  if folded
+                  then have_instruction_type_checker M F L body ψ L'
+                  else
+                    inr ([LocalCtxSynthError "your resulting locals aren't all nonrefs"
+                            L L' (combine_error_messages res)])
+                    (* inr ([NormalError "your resulting locals aren't all nonrefs"] ++ combine_error_messages res) *)
+                    (* INR ("your resulting locals aren't all norefs (" ++ *)
+                    (*           (combine_error_messages res) ++ ")"%string) *)
+              | inl None => INR "don't know how to deal with breaks and stuff yet for synthing local ctx"
+              | inr a => INR "error in synthing local ctx (e.g. bad local get/set)"
+              end
+          | None => INR "AAAAAAAAAAAAA"
+          end
+      | None => INR "aaaaaa"
+      end
+  | None => INR "can't give function type"
+  end.
+
+Fixpoint body_has_ifun_type_checker
+  (M : module_ctx)
+  (K : kind_ctx)
+  (mf_locs : list representation)
+  (body : list instruction)
+  (κs : list kind) (ϕ : inner_function_type)
+  : type_checker_res :=
+  match ϕ with
+  | MonoFunT τs1 τs2 => body_has_mono_type_checker M K mf_locs body κs τs1 τs2
+  | ForallTypeT κ ϕ => body_has_ifun_type_checker M K mf_locs body (κ :: κs) ϕ
+  end.
+
+Fixpoint body_has_fun_type_checker
+  (M : module_ctx)
+  (mf_locs : list representation)
+  (body : list instruction)
+  (K : kind_ctx)
+  (ϕ : function_type)
+  : type_checker_res :=
+  match ϕ with
+  | InnerFunT ϕ =>
+    body_has_ifun_type_checker M K mf_locs body [] ϕ
+  | ForallMemT ϕ =>
+    body_has_fun_type_checker M mf_locs body (K <| kc_mem_vars ::= S |>) ϕ
+  | ForallRepT ϕ =>
+    body_has_fun_type_checker M mf_locs body (K <| kc_rep_vars ::= S |>) ϕ
+  | ForallSizeT ϕ =>
+    body_has_fun_type_checker M mf_locs body (K <| kc_size_vars ::= S |>) ϕ
+  end.
+
 Definition has_function_type_checker
-    (M:module_ctx) (mf:module_function) (ft:function_type) : type_checker_res :=
-  if function_type_beq mf.(mf_type) ft
-  then
-    let ϕ := flatten_function_type mf.(mf_type) in
-    let K := kc_of_fft ϕ in
-    match mapM (eval_rep_prim EmptyEnv) mf.(mf_locals) with
-    | Some ηss_L =>
-        let tempF := Build_function_ctx [] [] [] K ϕ.(fft_type_vars) in
-        match mapM (grab_rep tempF) ϕ.(fft_in) with
-        | Some ρs_P =>
-            match mapM (eval_rep_prim EmptyEnv) ρs_P with
-            | Some ηss_P =>
-                let tempF2 := Build_function_ctx ϕ.(fft_out) (ηss_P ++ ηss_L) [] K ϕ.(fft_type_vars) in
-                let L := ϕ.(fft_in) ++ map type_plug_prim ηss_L in
-                let ψ := InstrT [] ϕ.(fft_out) in
-                match synth_possible_resulting_local_ctx_insts tempF2 (mf.(mf_body)) L with
-                | inl (Some L') =>
-                    let F := tempF2 <| fc_labels := [(ϕ.(fft_out), L')] |> in
-                    let res := map (λ t, has_ref_flag_checker F t NoRefs) L' in
-                    let folded := foldr (λ r, andb (check_ok_output r)) true res in
-                    if folded
-                    then have_instruction_type_checker M F L mf.(mf_body) ψ L'
-                    else
-                      inr ([LocalCtxSynthError "your resulting locals aren't all nonrefs"
-                              L L' (combine_error_messages res)])
-                      (* inr ([NormalError "your resulting locals aren't all nonrefs"] ++ combine_error_messages res) *)
-                      (* INR ("your resulting locals aren't all norefs (" ++ *)
-                      (*           (combine_error_messages res) ++ ")"%string) *)
-                | inl None => INR "don't know how to deal with breaks and stuff yet for synthing local ctx"
-                | inr a => INR "error in synthing local ctx (e.g. bad local get/set)"
-                end
-            | None => INR "AAAAAAAAAAAAA"
-            end
-        | None => INR "aaaaaa"
-        end
-    | None => INR "can't give function type"
-    end
-  else INR "bad".
+    (M:module_ctx) (mf:module_function) : type_checker_res :=
+  body_has_fun_type_checker M mf.(mf_locals) mf.(mf_body) kc_empty mf.(mf_type).
 
 
 Lemma grab_rep_in_messed_up_F :
@@ -5251,7 +5286,7 @@ Proof.
 Qed.
 
 Lemma has_function_type_checker_correct :
-  ∀ M mf, has_function_type_checker M mf mf.(mf_type) = ok_term ->
+  ∀ M mf, has_function_type_checker M mf = ok_term ->
           has_function_type M mf.
 Proof.
 Admitted.
@@ -5266,7 +5301,7 @@ Definition has_module_type_checker (m:module) (mt:module_type) : type_checker_re
           if module_type_beq mt (Build_module_type m.(m_imports) exports)
           then
             let M := Build_module_ctx ϕs table in
-            let res := map (λ mf, has_function_type_checker M mf mf.(mf_type)) m.(m_functions) in
+            let res := map (λ mf, has_function_type_checker M mf) m.(m_functions) in
             let folded := foldr (λ r, andb (check_ok_output r)) true res in
             if folded
             then ok_term
