theories/syntax.v
@@ -13,28 +13,6 @@ Inductive primitive :=
 
 Definition path : Type := list nat.
 
-Record flat_function_type :=
-  { fft_mem_vars : nat;
-    fft_rep_vars : nat;
-    fft_size_vars : nat;
-    fft_type_vars : list kind;
-    fft_in : list type;
-    fft_out : list type }.
-
-Fixpoint flatten_inner_function_type (ϕ : inner_function_type) : flat_function_type :=
-  match ϕ with
-  | MonoFunT τs1 τs2 => Build_flat_function_type 0 0 0 [] τs1 τs2
-  | ForallTypeT κ ϕ' => flatten_inner_function_type ϕ' <| fft_type_vars ::= app [κ] |>
-  end.
-
-Fixpoint flatten_function_type (ϕ : function_type) : flat_function_type :=
-  match ϕ with
-  | InnerFunT ϕ' => flatten_inner_function_type ϕ'
-  | ForallMemT ϕ' => flatten_function_type ϕ' <| fft_mem_vars ::= S |>
-  | ForallRepT ϕ' => flatten_function_type ϕ' <| fft_rep_vars ::= S |>
-  | ForallSizeT ϕ' => flatten_function_type ϕ' <| fft_size_vars ::= S |>
-  end.
-
 Definition arep_to_prim (ι : atomic_rep) : primitive :=
   match ι with
   | PtrR => I32P
